---
tags:
  - Maths/Algebraic_expressions
date: 2025-06-16
aliases:
  - expanding brackets
cssclasses:
  - neo-headings
  - bai-headings
  - rounded-images
  - pen-green
lang:
  - en
properties-ver: "1.1"
---
# Expanding brackets

***
## Expanding basic single brackets
To expand a simple bracket multiply the numbers in the bracket by the number outside the bracket. The basic formula is:

$$
a(b + c) = ab + ac
$$

For example:

$$
\begin{aligned}
3(x + 2) &= 3x + 3 \cdot 2 \\
&= 3x + 6
\end{aligned}
$$

Here are some other examples:
$$
\begin{aligned}
2(4x +5) &= 2 \cdot 4x + 2 \cdot 5 \\
&= 8x + 10 \\ \\
5(2x + 3) &= 5 \cdot 2x + 5 \cdot 3 \\
&= 10x + 15 \\
\end{aligned}
$$

## Expanding double brackets
To expand double brackets, its the same process as before but with two brackets. The formula is:
$$
\begin{aligned}
(a + b)(c + d) = ac + ad + bc + bd \\
(x + y)(x + z) = x^2 + xz + xy + yz \\
\end{aligned}
$$
For example:
$$
\begin{aligned}
(2x + 8)(x + 4) &= 2x \cdot x + 2x \cdot 4 + 8 \cdot x + 8 \cdot 4 \\
&= 2x^2 + 8x + 8x + 32 \\
\end{aligned}
$$

### Grid method to expanding brackets
Some people find it hard to expand brackets using the formula above, so they use the grid method. This method involves drawing a grid and filling in the products of the terms from each bracket.

$$
\begin{aligned}
(2x + 8)(x + 4) &=
\begin{array}{|c|c|c|}
\hline
\times & x & 4 \\
\hline
2x & 2x^2 & 8x \\
\hline
8 & 8x & 32 \\
\hline
\end{array} \\
2x^2 + 8x + 8x + 32 &= 2x^2 + 16x + 32
\end{aligned}
$$

Then you add up all the terms in the grid:

### Expanding more complex double brackets
When you have more complex double brackets, you can still use the same formula. For example:

$$
\begin{aligned}
(a + b)(c + d + e) &= ac + ad + ae + bc + bd + be \\
\end{aligned}
$$
We can simplify using [[Collecting like terms]] to make the result more manageable. For example:
$$

\begin{aligned}
(2x + 3)(x + 4 + 5) &= 2x \cdot x + 2x \cdot 4 + 2x \cdot 5 + 3 \cdot x + 3 \cdot 4 + 3 \cdot 5 \\
&= 2x^2 + 8x + 10x + 3x + 12 + 15 \\
&= 2x^2 + (8x + 10x + 3x) + (12 + 15) \\
&= 2x^2 + 21x + 27
\end{aligned}
$$


## Expanding brackets with subtraction
When you have a subtraction in the brackets, you can treat it like a negative number. The formula is:

$$
\begin{aligned}
a(b - c) &= ab - ac \\
3(x - 2) &= 3x - 3 \cdot 2 \\
&= 3x - 6
\end{aligned}
$$

## Expanding negative brackets
When you have a negative bracket, you can treat it like a negative number. The formula is:
$$
\begin{aligned}
a(b - c) &= ab - ac \\
a(b + c) &= ab + ac \\
a(-b + c) &= -ab + ac \\
a(-b - c) &= -ab - ac \\
\end{aligned}
$$

Example:

$$
\begin{aligned}
-3(x - 2) &= -3x + 3 \cdot 2 \\
&= -3x + 6 \\
&= -3x + 6 \\
-3(x + 2) &= -3x - 3 \cdot 2 \\
\end{aligned}
$$